code/experimental/P256/Hacl.Impl.Gen.fst
@@ -1,0 +1,150 @@
+module Hacl.Impl.Gen
+
+open FStar.HyperStack.All
+open FStar.HyperStack
+module ST = FStar.HyperStack.ST
+
+open Lib.IntTypes
+open Lib.Buffer
+
+open Hacl.Impl.Curve25519.Field64.Core
+open Hacl.Spec.P256.Core
+open Hacl.Spec.P256.Lemmas
+open Hacl.Spec.P256.Definitions
+ 
+open FStar.Math.Lemmas
+
+
+val add_carry: cin: uint64 -> x: uint64 -> y: uint64 -> result1: lbuffer uint64 (size 1) -> 
+  Stack uint64 
+    (requires fun h -> live h result1)
+    (ensures fun h0 _ h1 -> True)
+
+let add_carry cin x y result1 = 
+  let res1 = x +. cin in 
+  let c = if lt_u64 res1 cin then u64 1 else u64 0 in
+  let res = res1 +. y in
+  let c = if lt_u64 res res1 then c +. u64 1 else c in
+  Lib.Buffer.upd result1 (size 0) res;
+  c
+
+
+
+val sub_borrow: cin: uint64 -> x: uint64 -> y: uint64 -> result1: lbuffer uint64 (size 1) -> 
+  Stack uint64
+    (requires fun h -> live h result1)
+    (ensures fun h0 _ h1 -> True)
+
+let sub_borrow cin x y result1 = 
+  let open Hacl.Spec.Curve25519.Field64.Core in 
+  let res = x -. y -. cin in
+  let c =
+    if eq_u64 cin (u64 1) then
+      (if le_u64 x y then u64 1 else u64 0)
+    else
+      (if lt_u64 x y then u64 1 else u64 0) in
+  Lib.Buffer.upd result1 (size 0) res;
+  c
+
+
+
+inline_for_extraction noextract
+val shift_carry: x: uint64 -> cin: uint64{uint_v cin <=1} -> Tot (r: uint64)
+
+let shift_carry x cin = 
+  add (Lib.IntTypes.shift_left x (size 1)) cin
+
+
+
+#set-options "--z3rlimit 500" 
+val p256_add: arg1: felem -> arg2: felem ->  out: felem -> Stack unit 
+  (requires (fun h0 ->  
+    (let arg1_as_seq = as_seq h0 arg1 in let arg2_as_seq = as_seq h0 arg2 in 
+    felem_seq_as_nat arg1_as_seq < prime /\ felem_seq_as_nat arg2_as_seq < prime /\
+    live h0 out /\ live h0 arg1 /\ live h0 arg2))
+  )
+  (ensures (fun h0 _ h1 -> modifies1 out h0 h1 /\ 
+    (let arg1_as_seq = as_seq h0 arg1 in let arg2_as_seq = as_seq h0 arg2 in 
+    as_nat h1 out < prime (*/\ as_seq h1 out == felem_add_seq arg1_as_seq arg2_as_seq)) *) ))
+  )
+
+let p256_add arg1 arg2 out = 
+    push_frame();
+  let h0 = ST.get() in 
+
+  let a0 = index arg1 (size 0) in 
+  let a1 = index arg1 (size 1) in 
+  let a2 = index arg1 (size 2) in 
+  let a3 = index arg1 (size 3) in 
+
+  let b0 = index arg2 (size 0) in 
+  let b1 = index arg2 (size 1) in 
+  let b2 = index arg2 (size 2) in 
+  let b3 = index arg2 (size 3) in 
+
+  let r0 = sub out (size 0) (size 1) in 
+  let r1 = sub out (size 1) (size 1) in 
+  let r2 = sub out (size 2) (size 1) in 
+  let r3 = sub out (size 3) (size 1) in 
+  
+  let cc = add_carry (u64 0) a0 b0 r0 in 
+  let cc = add_carry cc a1 b1 r1 in 
+  let cc = add_carry cc a2 b2 r2 in 
+  let cc = add_carry cc a3 b3 r3 in 
+
+  let t = cc in 
+  let cc = add_carry cc (index out (size 0)) (u64 0) r0 in 
+  let cc = add_carry cc (index out (size 1)) ((u64 0) -. (t <<. (size 32))) r1 in 
+  let cc = add_carry cc (index out (size 2)) ((u64 0) -. t) r2 in 
+  let _  = add_carry cc (index out (size 3)) ((t <<. (size 32)) -. (t <<. (size 1))) r3 in 
+
+
+  let h1 = ST.get() in 
+  pop_frame();
+  admit();
+  (*assert(Lib.Sequence.equal (as_seq h1 out) (felem_add_seq (as_seq h0 arg1) (as_seq h0 arg2)));*)
+  ()
+
+
+val p256_sub: arg1: felem -> arg2: felem -> out: felem -> Stack unit 
+  (requires 
+    (fun h0 -> live h0 out /\ live h0 arg1 /\ live h0 arg2 /\ as_nat h0 arg1 < prime /\ as_nat h0 arg2 < prime))
+  (ensures 
+    (fun h0 _ h1 ->modifies1 out h0 h1 /\  as_nat h1 out < prime ))
+
+let p256_sub arg1 arg2 out = 
+  let h0 = ST.get() in 
+        push_frame();
+  let h0 = ST.get() in 
+
+  let a0 = index arg1 (size 0) in 
+  let a1 = index arg1 (size 1) in 
+  let a2 = index arg1 (size 2) in 
+  let a3 = index arg1 (size 3) in 
+
+  let b0 = index arg2 (size 0) in 
+  let b1 = index arg2 (size 1) in 
+  let b2 = index arg2 (size 2) in 
+  let b3 = index arg2 (size 3) in 
+
+  let r0 = sub out (size 0) (size 1) in 
+  let r1 = sub out (size 1) (size 1) in 
+  let r2 = sub out (size 2) (size 1) in 
+  let r3 = sub out (size 3) (size 1) in 
+
+
+  let cc = sub_borrow (u64 0) a0 b0 r0 in 
+  let cc = sub_borrow cc a1 b1 r1 in 
+  let cc = sub_borrow cc a2 b2 r2 in 
+  let cc = sub_borrow cc a3 b3 r3 in 
+
+  let t = cc in 
+  let cc = add_carry (u64 0) (index out (size 0)) ((u64 0) -. t) r0 in 
+  let cc = add_carry cc (index out (size 1)) (((u64 0) -. t) >>. (size 32)) r1 in 
+  let cc = add_carry cc (index out (size 2)) (u64 0) r2 in 
+  let _ = add_carry cc (index out (size 3)) (t -. (t <<. (size 32))) r3 in 
+
+admit();
+    let h1 = ST.get() in 
+    pop_frame();
+  ()
